\subsection{Покоординатная сходимость в $\mathbb{R}^d$}
    \[ x_n = <x_n^{(1)}, \dots, x_n^{(d)}> \]
    $x_n$ покоординатно сходится к $x_0$, если \\
    \begin{gather*}
        \begin{cases}
            \lim x_n^{(1)} = x_0^{(1)} \\
            \dots \\
            \lim x_n^{(d)} = x_0^{(d)}
        \end{cases}
    \end{gather*}
    
    \begin{theorem-non} \end{theorem-non}
    $x_n$ покоординатно сходится к $x_0 \Longleftrightarrow x_n$ сходится к $x_0$ по норме в $\mathbb{R}^d$ 
    
    $||a|| = \sqrt{a_1^2 + \dots + a_d^2}$ - норма
    
    \begin{proof}
        \[ ||x_n - x_0|| = \sqrt{(x_n^{(1)} - x_0^{(1)})^2 + \dots + (x_n^{(d)} - x_0^{(d)})^2} \]
        Заметим следующее: 
        \[ \sqrt{(x_n^{(1)} - x_0^{(1)})^2 + \dots + (x_n^{(d)} - x_0^{(d)})^2} \geqslant \sqrt{(x_n^{(k)} - x_0^{(k)})^2} = |x_n^{(k)} - x_0^{(k)}| \]
        \[  \sqrt{(x_n^{(1)} - x_0^{(1)})^2 + \dots + (x_n^{(d)} - x_0^{(d)})^2} \leqslant |x_n^{(1)} - x_0^{(1)}| + \dots + |x_n^{(d)} - x_0^{(d)}| \]
        Итого получаем
        \[ |x_n^{(k)} - x_0^{(k)}| \leqslant ||x_n - x_0|| \leqslant |x_n^{(1)} - x_0^{(1)}| + \dots + |x_n^{(d)} - x_0^{(d)}| \]
        Докажем $"\Leftarrow"$:
        \[ \lim x_n = x_0 \Rightarrow ||x_n - x_0|| \to 0 \Rightarrow  |x_n^{(k)} - x_0^{(k)}| \to 0 \Rightarrow \lim x_n^{(k)} = x_0^{(k)} \]
        Докажем $"\Rightarrow"$:
        \[ \lim x_n^{(k)} = x_0^{(k)} \Rightarrow |x_n^{(k)} - x_0^{(k)}| \to 0 \Rightarrow \sum_{k = 1}^d |x_n^{(k)} - x_0^{(k)}| \to 0 \Rightarrow ||x_n - x_0|| \to 0 \Rightarrow \lim x_n = x_0  \]
    \end{proof}